CSR sum wip

CSR.v
@@ -1,6 +1,6 @@
 Set Implicit Arguments.
 From SLF Require Import LabType Fun LibSepFmap Sum.
-From SLF Require Import LibSepReference LibSepTLCbuffer Struct Unary_IndexWithBounds Loops.
+From SLF Require Import LibSepReference LibSepTLCbuffer Struct Unary_IndexWithBounds Loops SV2.
 From mathcomp Require Import ssreflect ssrfun zify.
 Hint Rewrite conseq_cons' : rew_listx.
 
@@ -14,9 +14,11 @@ Definition to_int (v : val) : int :=
 
 Coercion to_int : val >-> Z.
 
-Module Export AD := WithUnary(Int2Dom).
+(* Module Export AD := WithUnary(Int2Dom). *)
 
 Module csr.
+
+Import sv.
 
 Section csr.
 
@@ -34,6 +36,7 @@ Import List Vars.
 
 Context (mval colind rowptr : list int).
 Context (N Nrow Ncol : int).
+Hypothesis Nrow_nonneg : 0 <= Nrow.
 Hypothesis len_mval : length mval = N :> int.
 Hypothesis len_colind : length colind = N :> int.
 Hypothesis len_rowptr : length rowptr = Nrow + 1 :> int.
@@ -57,12 +60,15 @@ Tactic Notation "seclocal_solver" :=
   first [ assumption 
     | rewrite -/(colind_seg _); now apply nodup_eachcol
     | (* for rowptr[?] <= N *)
-      try rewrite -> len_colind; try rewrite <- rowptr_last; apply rowptr_weakly_sorted; math
+      try rewrite -> len_colind; try rewrite -> len_mval; 
+      try rewrite <- rowptr_last; apply rowptr_weakly_sorted; math
+    | (* for 0 <= rowptr[?] *)
+      rewrite <- rowptr_first at 1; apply rowptr_weakly_sorted; math
     | (* for 0 <= rowptr[i] <= rowptr[i + 1] *)
       split; [ rewrite <- rowptr_first at 1 | ]; apply rowptr_weakly_sorted; math
     | idtac ]; auto.
 
-Definition indexf := index_bounded.func.
+(* Definition indexf := index_bounded.func. *)
 
 Definition csrij := 
 <{
@@ -70,12 +76,13 @@ Definition csrij :=
     let "lb" = read_array rowptr i in
     let "ii" = i + 1 in
     let "rb" = read_array rowptr "ii" in
-    let k = indexf "lb" "rb" j colind in
+    (* let k = indexf "lb" "rb" j colind in
     let c = k < "rb" in
     if c
     then 
       let "tmp" = read_array mval k in "tmp"
-    else 0
+    else 0 *)
+    sv.get j colind mval "lb" "rb"
 }>.
 
 Lemma csrij_spec_in `{Inhab D} (x_mval x_colind x_rowptr : loc) (i j : int) d : 
@@ -94,11 +101,9 @@ Lemma csrij_spec_in `{Inhab D} (x_mval x_colind x_rowptr : loc) (i j : int) d :
 Proof with seclocal_solver.
   rewrite -wp_equiv; xsimpl=> ??.
   do 3 (xwp; xapp).
-  xwp; xapp index_bounded.spec=> //...
-  rewrite /colind_seg index_nodup...
-  2: rewrite list_interval_length...
-  xwp; xapp. xwp; xif=> ?; try math. 
-  xwp; xapp. xwp; xval. xsimpl*.
+  rewrite /colind_seg.
+  xapp get_spec_in; eauto... 
+  rewrite <- list_interval_nth... xsimpl*.
 Qed.
 
 Lemma csrij_spec_out_unary `{Inhab D} (x_mval x_colind x_rowptr : loc) (i j : int) d :
@@ -114,14 +119,14 @@ Lemma csrij_spec_out_unary `{Inhab D} (x_mval x_colind x_rowptr : loc) (i j : in
       harray_int colind x_colind d \* 
       harray_int rowptr x_rowptr d).
 Proof with seclocal_solver.
-  rewrite -wp_equiv; xsimpl.
-  intros (? & HH%memNindex). 
+  rewrite -wp_equiv; xsimpl=> ?.
   do 3 (xwp; xapp).
-  xwp; xapp index_bounded.spec=> //...
-  rewrite -/(colind_seg _) HH list_interval_length...
-  xwp; xapp. xwp; xif=> ?; try math. xwp; xval. xsimpl*.
+  xapp get_spec_out_unary; eauto...
+  1: now unfold colind_seg in *.
+  xsimpl*.
 Qed.
 
+(* here lb and rb are not fixed, so cannot directly apply get_spec_out *)
 Lemma csrij_spec_out `{Inhab D} fs (x_mval x_colind x_rowptr : loc) : 
   htriple fs
     (fun d => csrij x_mval x_colind x_rowptr (eld d).1 (eld d).2)
@@ -146,10 +151,19 @@ Qed.
 
 Definition csrsum := 
   <{
-  fun mval =>
+  fun mval colind rowptr =>
   let s = ref 0 in
+  (* 
   for i <- [0, N] {
     let x = mval[i] in 
+    s += x
+  }; 
+  *)
+  for i <- [0, Nrow] {
+    let "lb" = read_array rowptr i in
+    let "ii" = i + 1 in
+    let "rb" = read_array rowptr "ii" in
+    let x = sv.sum colind mval "lb" "rb" in 
     s += x
   };
   ! s
@@ -160,8 +174,6 @@ Tactic Notation "seclocal_fold" :=
     -/(For_aux _ _) 
     -/(For _ _ _) //=.
 
-Lemma Union_depprod_collapse : 
-
 Lemma csrsum_spec `{Inhab D} (x_mval x_colind x_rowptr : loc) : 
   {{ arr(x_mval, mval)⟨1, (0,0)⟩ \*
      arr(x_colind, colind)⟨1, (0,0)⟩ \*
@@ -170,74 +182,24 @@ Lemma csrsum_spec `{Inhab D} (x_mval x_colind x_rowptr : loc) :
      (\*_(i <- `[0, Nrow] \x `[0, Ncol]) arr(x_colind, colind)⟨2, i⟩) \*
      (\*_(i <- `[0, Nrow] \x `[0, Ncol]) arr(x_rowptr, rowptr)⟨2, i⟩) }}
   [{
-    [1| ld in `{(0,0)}   => csrsum x_mval];
+    [1| ld in `{(0,0)}   => csrsum x_mval x_colind x_rowptr];
     {2| ld in `[0, Nrow] \x `[0, Ncol] => csrij x_mval x_colind x_rowptr ld.1 ld.2}
   }]
   {{ hv, \[hv[`1]((0,0)) = Σ_(i <- `[0, Nrow] \x `[0, Ncol]) hv[`2](i)] \* \Top}}.
 Proof with (try seclocal_fold; seclocal_solver).
-  set (is_valid_coor := (fun rc : int * int => 0 <= rc.1 < Nrow /\ In rc.2 (colind_seg rc.1))).
-  xfocus (2,0) is_valid_coor.
-  rewrite (hbig_fset_part (`[0, Nrow] \x `[0, Ncol]) is_valid_coor). (* TODO: there is a todo in COO here *)
-  xapp csrij_spec_out=> //.
-  { case=> ?? /[! @indom_label_eq]-[_]/=. 
-    rewrite /is_valid_coor /intr filter_indom indom_prod indom_interval; autos*. }
-  set (H1 := hbig_fset hstar (_ ∖ _) _); 
-  set (H2 := hbig_fset hstar (_ ∖ _) _);
-  set (H3 := hbig_fset hstar (_ ∖ _) _).
-  xframe (H1 \* H2 \* H3); clear H1 H2 H3.
-  (* TODO this is not a good proof, though; a more natural way is to split the For loop? *)
-  (* TODO need some segmentation *)
-  have E : (`[0, Nrow] \x `[0, Ncol]) ∩ is_valid_coor = 
-    Union (interval 0 Nrow) (fun i => Union (interval (nth (abs i) rowptr 0) (nth (abs (i + 1)) rowptr 0)) 
-      (fun j => single (i, nth (abs j) colind 0) tt)).
-  { subst is_valid_coor. apply fset_extens. intros (r, c).
-    rewrite /intr /colind_seg filter_indom indom_prod indom_Union ?indom_interval //=.
+  xin (1,0) : xwp; xapp=> s...
+  xin (2,0) : do 3 (xwp; xapp).
+  (* TODO extract this to be a lemma *)
+  assert (`[0, Nrow] \x `[0, Ncol] = Union `[0, Nrow] (fun i => `{i} \x `[0, Ncol])) as E.
+  { apply fset_extens. intros (r, c).
+    rewrite indom_prod indom_Union !indom_interval /=.
     split.
-    { intros ((Hr & Hc) & _ & Hin).
-      exists r.
-      rewrite indom_interval. split; auto. 
-      rewrite indom_Union.
-      pose proof Hin as Hin'%(nth_index 0).
-      rewrite <- index_mem, -> list_interval_length in Hin...
-      set (idx := index _ _) in Hin, Hin'.
-      assert (0 <= idx) by (subst idx; apply indexG0).
-      exists ((nth (abs r) rowptr 0) + idx).
-      rewrite indom_interval indom_single_eq. 
-      rewrite -> list_interval_nth with (lb:=(nth (abs r) rowptr 0)) (rb:=(nth (abs (r + 1)) rowptr 0))...
-      rewrite Hin'. split; try math; auto. }
-    { intros (r' & Hr' & HH).
-      rewrite indom_Union in HH. destruct HH as (c' & Hc' & HH).
-      rewrite -> indom_interval in Hr', Hc'. rewrite indom_single_eq in HH.
-      injection HH as <-. subst c.
-      admit.
-    }
+    { intros (Hr & Hc). exists r. 
+      rewrite indom_prod !indom_interval indom_single_eq //=. }
+    { intros (f & Hq). 
+      rewrite indom_prod !indom_interval indom_single_eq /= in Hq. eqsolve. }
   }
   rewrite E.
-
-
-      assert (0 <= (nth (abs r') rowptr 0) <= (nth (abs (r' + 1)) rowptr 0)) as HH1...
-      assert ((nth (abs (r' + 1)) rowptr 0) <= N) as HH2...
-      assert (abs c' < Datatypes.length colind)%nat as HH3 by math.
-      apply nth_In with (d:=0) in HH3.
-      
-      nth In
-
-
-       
-
-      
-      
-      
-
-
-    simpl.
-    setoid_rewrite indom_interval.
-    setoid_rewrite indom_Union.
-    setoid_rewrite indom_interval.
-    setoid_rewrite indom_single_eq.
-    
-
-  xin (1,0) : xwp; xapp=> s...
   set (R i := 
     arr(x_mval, mval)⟨2, i⟩ \*
     arr(x_colind, colind)⟨2, i⟩ \* 
@@ -246,48 +208,23 @@ Proof with (try seclocal_fold; seclocal_solver).
     arr(x_mval, mval)⟨1, (0,0)⟩ \* 
     arr(x_colind, colind)⟨1, (0,0)⟩ \* 
     arr(x_rowptr, rowptr)⟨1, (0,0)⟩).
-
-    For
-  xfor_sum Inv R (fun=> \Top) (fun hv i => hv[`2]((xrow[i], xcol[i]))) s.
-  xfor_big_op_lemma
-
-  
-  have E : (`[0, Nrow] \x `[0, Ncol]) ∩ is_valid_coor = is_valid_coor.
-
-  
-
-  xin (1,0) : xwp; xapp=> s...
-  { apply/fset_extens=> -[??]. 
-    rewrite /intr filter_indom indom_prod -fset_of_list_in; splits*.
-    rewrite /Sum.mem in_combineE /= ?indom_interval=> -[]; autos*. }
-  rewrite ?E (fset_of_list_nodup (0,0)) // lE.
-  set (R i := 
-    arr(x_row, xrow)⟨2, i⟩ \*
-    arr(x_col, xcol)⟨2, i⟩ \* 
-    arr(x_val, xval)⟨2, i⟩).
-  set (Inv (i : int) := 
-    arr(x_row, xrow)⟨1, (0,0)⟩ \* 
-    arr(x_col, xcol)⟨1, (0,0)⟩ \* 
-    arr(x_val, xval)⟨1, (0,0)⟩).
-  xfor_sum Inv R (fun=> \Top) (fun hv i => hv[`2]((xrow[i], xcol[i]))) s.
+  xin (1,0) : idtac... (* making 1 be above 2 *)
+  xfor_sum Inv R (fun=> \Top) (fun hv i => Σ_(j <- `{i} \x `[0, Ncol]) hv[`2](j)) s.
   { rewrite /Inv /R.
-    (xin (1,0): (xwp; xapp; xapp incr.spec=> y))...
-    rewrite ?combine_nth /=; try lia.
-    xapp get_spec_in=> //; xsimpl*. }
-  { move=> Neq ???; apply/Neq. 
-    move/NoDup_nthZ: nodup_xrowcol; apply; autos*; math. }
-  { rewrite combine_nth //; lia. }
-  { lia. }
-  xapp; xsimpl.
-  under (@SumEq _ _ _ (`[0, Nrow] \x `[0, Ncol])).
-  { move=>*; rewrite to_int_if; over. }
-  rewrite SumIf E (SumList (0,0)) // lE Sum0s.
-  under (@SumEq _ _ _ `[0,N]).
-  { move=> ?; rewrite -combine_nth; last lia. over. }
-  math.
-Qed.
-
-
+    xin (1,0) : do 3 (xwp; xapp)...
+    xframe2 (arr(x_rowptr, rowptr)⟨1, (0, 0)⟩). xsimpl.
+    xin (1,0) : idtac. (* format fix *)
+    admit. (* how to use the spec of sv.sum here? *)
+  }
+  { intros Hneq Hi Hj. 
+    apply disjoint_of_not_indom_both.
+    intros (r, c). rewrite !indom_prod !indom_interval !indom_single_eq /=. math. }
+  { xapp. xsimpl*. rewrite SumCascade; try reflexivity.
+    (* repeating the proof above? *)
+    intros i0 j0 Hneq. rewrite ! indom_interval=> ? ?.
+    apply disjoint_of_not_indom_both.
+    intros (r, c). rewrite !indom_prod !indom_interval !indom_single_eq /=. math. }
+Abort.
 
 End csr.
 
